

Topics in Number Theory

Instructor : Dr. Kaneenika Sinha

Spring 2026

Contents

1	Elementary Methods	1
1.1	Arithmetic Functions	1
1.2	Infinite Products	3
1.3	Ordering of Arithmetical Functions	5
1.4	Summation Tools	7
1.5	Finite Abelian Groups	7
2	Analytic Theory	9
3	Advanced Topics	10

Chapter 1

Elementary Methods

1.1 Arithmetic Functions

Definition 1.1. A function is said to be arithmetic, if $f : \mathbb{N} \rightarrow \mathbb{C}$.

- f is said to be additive if $f(mn) = f(m) + f(n) \forall m, n$ such that $(m, n) = 1$.
- f is said to be multiplicative if $f(mn) = f(m)f(n) \forall m, n$ such that $(m, n) = 1$.
- f is said to be completely additive or multiplicative if additive or multiplicative property holds for all $m, n \in \mathbb{N}$

Examples. Some arithmetic functions:

1. $\omega : \mathbb{N} \rightarrow \mathbb{C}, \omega(n) = \# \text{distinct prime factors of } n$.
Additive.
2. $\Omega : \mathbb{N} \rightarrow \mathbb{C}, \Omega(n) = \# \text{prime factors of } n \text{ with multiplicity}$.
Completely additive.
3. $\log : \mathbb{N} \rightarrow \mathbb{C}$
Completely additive.
4. $\mu : \mathbb{N} \rightarrow \mathbb{C}$ - Mobius function

$$\mu(n) = \begin{cases} (-1)^{\omega(n)} & n \text{ is squarefree} \\ 0 & \text{otherwise} \end{cases}$$

Multiplicative.

5. $\Lambda : \mathbb{N} \rightarrow \mathbb{C}$ - von Mangoldt function

$$\Lambda(n) = \begin{cases} \log(p) & \text{if } n = p^\alpha \text{ for some prime } p \\ 0 & \text{otherwise} \end{cases}$$

Neither multiplicative nor additive.

6. $\lambda(n) : \mathbb{N} \rightarrow \mathbb{C}$ - Liouville's function

$$\lambda(n) = \begin{cases} 1 & n = 1 \\ (-1)^{\alpha_1 + \alpha_2 + \dots + \alpha_k} & \alpha_i \text{ such that } n = \prod_{i \leq k} p_i^{\alpha_i} \end{cases}$$

Completely multiplicative.

7. $\varphi : \mathbb{N} \rightarrow \mathbb{C}$ - Euler's totient function

$$\begin{aligned} \varphi(n) &= |\{1 \leq k \leq n : (n, k) = 1\}| \\ &= n \prod_{p|n} \left(1 - \frac{1}{p}\right), \text{ and } \varphi(1) = 1. \end{aligned}$$

$$\varphi(mn) = \varphi(m)\varphi(n) \frac{(m,n)}{\varphi(m,n)}$$

8. $f : \mathbb{N} \rightarrow \mathbb{C}, f(n) = n^{-s}, s \in \mathbb{C}$.

Completely multiplicative.

Theorem 1.1. If $n \geq 1$, $\sum_{d|n} \mu(d) = I(n) := \begin{cases} 1 & n=1 \\ 0 & n>1 \end{cases}$.

Proof. When $n = 1$, the summation is equal to $1 = I(1)$. Let $n = \prod_{i=1}^m p_i^{\alpha_i}$ for

some $m \in \mathbb{N}$, and let $N = \prod_{i=1}^m p_i$. Now,

$$\begin{aligned} \sum_{d|n} \mu(d) &= \sum_{d|N} \mu(d) = 1 + \sum_{1 \leq i \leq m} \mu(p_i) + \sum_{1 \leq i, j \leq m} \mu(p_i p_j) + \dots + \mu(N) \\ &= 1 - \binom{m}{1} + \binom{m}{2} - \dots + (-1)^m \\ &= (1 + (-1))^m = 0 = I(n) \end{aligned}$$

■

Definition 1.2 (Number Field). A finite field extension of \mathbb{Q} is known as a number field.

Definition 1.3. An integer α is said to be algebraic if $f(\alpha) = 0$ for some monic irreducible $f \in \mathbb{Z}[x]$.

Definition 1.4. Given a number field K , the set

$$\theta_K := \{\alpha \in K : \alpha \text{ is an algebraic integer}\}$$

is known as its ring of integers.

Theorem 1.2. Given $\zeta(s) > 0 \forall s > 1$, there are infinitely many primes.

Proof. By Euler product formula,

$$\begin{aligned} \log \zeta(s) &= \sum_p \log \left(1 - \frac{1}{p^s} \right) = \sum_p \sum_{n=1}^{\infty} \frac{1}{np^{ns}} \\ &= \sum_p \frac{1}{p^s} + \sum_p \sum_{n \geq 2} \frac{1}{np^{ns}} \end{aligned}$$

If $s > 1$,

$$\begin{aligned} \sum_p \sum_{n \geq 2} \frac{1}{np^{ns}} &\leq \sum_p \sum_{n \geq 2} \frac{1}{p^n} \\ &= \sum_p \frac{1}{p(p-1)} \leq \sum_p \frac{2}{p^2} < \infty \\ \implies \lim_{s \rightarrow 1^+} \log \zeta(s) &= +\infty \\ \implies \sum_p \frac{1}{p} &= +\infty \end{aligned}$$

Hence, there are infinitely many primes. ■

1.2 Infinite Products

Let $\alpha_1, \alpha_2, \dots$ be a sequence in \mathbb{R} , and let $P(n) = \prod_{k=1}^n \alpha_k$. If $\lim_{n \rightarrow \infty} \prod_{k=1}^n \alpha_k$ converges, then we say that $\prod_{k=1}^{\infty} \alpha_k$ converges.

If $\prod_{k=1}^{\infty} (1 + a_k)$ converges, then $\forall k, a_k \neq -1$, and for all $k \geq 2$,

$1 + a_k = \frac{p(k)}{p(k-1)} \implies \lim_{k \rightarrow \infty} (1 + a_k) = 1$. Thus, if $\prod_{k=1}^{\infty} (1 + a_k)$ converges, then $\lim_{k \rightarrow \infty} a_k = 0$

Theorem 1.3. Given $a_k \geq 0 \forall k \geq 1$, $\prod_{k=1}^{\infty} (a_k + 1)$ converges iff $\sum_{k=1}^{\infty} a_k < \infty$.

Proof. Let $S(n) := \sum_{k=1}^n a_k$, and $p(n) := \prod_{k=1}^n (1 + a_k)$.

$$\begin{aligned} 0 \leq \sum_{k=1}^n a_k &\leq \prod_{k=1}^n (1 + a_k) \\ &\leq \prod_{k=1}^n e^{a_k} \\ &= e^{\left(\sum_{k=1}^n a_k\right)} \end{aligned}$$

$$\implies 0 \leq S(n) \leq p(n) \leq e^{S(n)}$$

Since both $S(n)$ and $p(n)$ are monotonically increasing, $\lim_{n \rightarrow \infty} p(n)$ exists iff $\lim_{n \rightarrow \infty} S(n)$ exists and is nonzero. ■

Corollary. $\prod_{k=1}^{\infty} (1 + |a_k|) < \infty \Leftrightarrow \sum_{k=1}^{\infty} |a_k| < \infty$.

Theorem 1.4. If $\prod_{k=1}^{\infty} (1 + |a_k|)$ converges, then $\prod_{k=1}^{\infty} (1 + a_k)$ also converges.

Proof. Let $P(n) = \prod_{k=1}^n (1 + a_k)$, and $R(n) = \prod_{k=1}^n (1 + |a_k|)$.

$\sum_{n=2}^{\infty} (R(n) - R(n-1)) < \infty$, since it is given that $\{R(n)\}_{n \geq 2}$ converges.

Now,

$$\begin{aligned}
0 \leq |P(n) - P(n-1)| &= |a_n P(n-1)| \\
&= \left| a_n \prod_{k=1}^{n-1} (1 + a_k) \right| \\
&\leq |a_n| \prod_{k=1}^{n-1} (1 + |a_k|) \\
&= R(n) - R(n-1)
\end{aligned}$$

$$\therefore \sum_{n=2}^{\infty} |P(n) - P(n-1)| < \infty \implies \sum_{n=2}^{\infty} P(n) - P(n-1) < \infty$$

Further,

$$\begin{aligned}
\sum_{n=2}^{\infty} P(n) - P(n-1) &= \lim_{n \rightarrow \infty} P(n) - P(1) \\
&\implies \lim_{n \rightarrow \infty} P(n) < \infty
\end{aligned}$$

Since $a_k \rightarrow 0$ as $k \rightarrow \infty$, $|1 + a_k| \leq \frac{1}{2}$ for all $k \geq k_0$, for some large k_0 ,

$$\begin{aligned}
&\forall k \geq k_0, \left| \frac{-a_k}{1 + a_k} \right| \leq 2|a_k| \\
&\implies \prod_{k=1}^{\infty} \left(1 - \frac{a_k}{a_{k+1}} \right) < \infty \\
&\implies \prod_{k=1}^{\infty} \left(\frac{1}{1 + a_k} \right) < \infty
\end{aligned}$$

Hence, $\lim_{n \rightarrow \infty} P(n) \neq 0$ ■

1.3 Ordering of Arithmetical Functions

Definition 1.5. Take $f : \mathbb{R} \rightarrow \mathbb{C}$, and consider $g : \mathbb{R} \rightarrow \mathbb{R}$ such that $g(x) > 0$ for all $x \geq x_0$ for some $x_0 \in \mathbb{R}$.

→ If $\exists C > 0$ such that $|f(x)| \leq Cg(x)$ for all $x \geq x_0$ or as $x \rightarrow \infty$, we say $f \ll g$, and that $f = O(g)$.

→ If $\exists C > 0$ such that $|f(x)| \geq Cg(x)$ for all $x \geq x_0$ or as $x \rightarrow \infty$, we say $f \gg g$.

Definition 1.6. Given $f : \mathbb{N} \rightarrow \mathbb{C}$, and $g : \mathbb{R} \rightarrow \mathbb{R}$ such that $g(x) > 0$ for all $x \geq x_0$ for some $x_0 \in \mathbb{R}$, we say that $f = o(g)$ (as $n \rightarrow \infty$), if $\lim_{n \rightarrow \infty} \frac{f(n)}{g(n)} = 0$.
 $f = o(g) \implies f = O(g)$.

Proposition 1.1. $\log(n) = O(n^\epsilon)$, for all $\epsilon > 0$.

Proof. Let $g : [1, \infty) \rightarrow \mathbb{R}$, such that $g(x) = \frac{\log(x)}{x^\epsilon}$.

$$\begin{aligned} g'(x) = 0 &\implies \frac{x^{\epsilon-1} - \epsilon \log(x) x^{\epsilon-1}}{x^{2\epsilon}} = 0 \\ &\implies \epsilon \log(x) = 1 \\ &\implies x = e^{\frac{1}{\epsilon}} \end{aligned}$$

That is, for all $x \geq 1$

$$\begin{aligned} g(x) &\leq g(e^{\frac{1}{\epsilon}}) = \frac{1}{e^\epsilon} \\ &\implies \log(x) \leq \frac{x^\epsilon}{e^\epsilon} \end{aligned}$$

■

Proposition 1.2. $d(n) = O(n^\epsilon)$, where $d(n) := \#$ of positive divisors of n .

Proof. We know that $n = \prod_{p|n} p^{\alpha_p}$. Let $a|n$; then $a = \prod_{p|n} p^{b_p}$, where $0 \leq b_p \leq \alpha_p$. Thus, $d(n) = \prod_{p|n} (\alpha_p + 1)$.

$$\begin{aligned} \frac{d(n)}{n^\epsilon} &= \prod_{p|n} \frac{\alpha_p + 1}{p^{\alpha_p \epsilon}} \\ &= \prod_{\substack{p|n \\ p < 2^{1/\epsilon}}} \frac{\alpha_p + 1}{p^{\alpha_p \epsilon}} \prod_{\substack{p|n \\ p \geq 2^{1/\epsilon}}} \frac{\alpha_p + 1}{p^{\alpha_p \epsilon}} \end{aligned}$$

When $\epsilon \geq 1$, it is easy to see that the proposition holds. Now we consider $0 < \epsilon \leq 1$. Note that $\prod_{\substack{p|n \\ p \geq 2^{1/\epsilon}}} \frac{\alpha_p + 1}{p^{\alpha_p \epsilon}}$ has factors $\frac{\alpha_p + 1}{p^{\alpha_p \epsilon}} \leq \frac{\alpha_p + 1}{2^{\alpha_p \epsilon}} \leq 1$.

$$\implies \frac{d(n)}{n^\epsilon} \leq \prod_{p < 2^{1/\epsilon}} < \prod_{\substack{p|n \\ p < 2^{1/\epsilon}}} \frac{\alpha_p + 1}{p^{\alpha_p \epsilon}}$$

Now since $p < 2^{1/\varepsilon}$,

$$\frac{\alpha_p + 1}{p^{\alpha_p \varepsilon}} \leq 1 + \frac{\alpha_p}{p^{\alpha_p \varepsilon}} \leq 1 + \frac{1}{\varepsilon \log p}$$

Hence,

$$\frac{d(n)}{n^\varepsilon} \leq \prod_{p < 2^{1/\varepsilon}} \left(1 + \frac{1}{\varepsilon \log p}\right) \implies d(n) \leq C(\varepsilon) n^\varepsilon$$

■

Theorem 1.5. $\forall \delta > 0 \exists n_0 \in \mathbb{N}$, such that $d(n) < 2^{(1+\delta) \frac{\log n}{\log \log n}}$, $\forall n \geq n_0$

Proved in [Murty, 2008] Ex. 1.33

Remark. $2^{\omega(n)} \leq n$, as $\omega(n) \leq \frac{\log n}{\log 2}$, that is $\omega(n) = O(n)$. Further, $2^{\omega(n)} \leq d(n)$ gives $\omega(n) \leq \frac{\log d(n)}{\log 2}$, which implies that $\omega(n) \ll \frac{\log n}{\log \log n}$.

1.4 Summation Tools

1.4.1 Abel Summation

1.5 Finite Abelian Groups

Definition 1.7. A function of the form $\chi : G \rightarrow S^1$ such that $\chi(ab) = \chi(a)\chi(b)$ for all $a, b \in G$, where G is a finite abelian group is known as a character.

The set of all characters of G is usually denoted as \widehat{G} . It can be shown that \widehat{G} is a group with the binary operation $\chi\psi(g) := \chi(g)\psi(g)$. The trivial character χ_0 such that $\chi_0(g) = 1$ for all $g \in G$ will act as the identity of the group. The group \widehat{G} will be abelian if G is abelian.

Proposition 1.3. If $f \in \widehat{G}$, then $f = e_l$ for some $l \in G$, where $e_l(k) := e^{2\pi i \frac{lk}{q}}$ for $G = \mathbb{Z}/q\mathbb{Z}$.

Lemma 1.1. Suppose $e : G \rightarrow \mathbb{C}^\times$ is a function such that $e(ab) = e(a)e(b)$ for all $a, b \in G$. Then $e \in \widehat{G}$.

Proof. Let $|G| = n$. We know that $e(a^n) = 1$ for all $a \in G$. Hence $|e(a) - 1| = 0$ for all $a \in G$. ■

Lemma 1.2. If $e \in \widehat{G}$ is not the identity, then $\sum_{a \in G} e(a) = 0$.

Proof. Choose a $b \in G$ such that $e(b) \neq 0$.

$$\begin{aligned}
 e(b) \sum_{a \in G} e(a) &= \sum_{a \in G} e(ab) \\
 &= \sum_{a \in G} e(a) \\
 \implies (e(b) - 1) \sum_{a \in G} e(a) &= 0 \\
 \implies \sum_{a \in G} e(a) &= 0
 \end{aligned}$$

■

Let $V = \{f : G \rightarrow \mathbb{C}\}$. V forms a finite dimensional vector space over \mathbb{C} . Define inner product on V : $\langle f_1, f_2 \rangle := \frac{1}{|G|} \sum_{a \in G} f_1(a) \overline{f_2(a)}$

Theorem 1.6. \widehat{G} forms an orthonormal set in V .

Proof. For any $e_l, e_k \in \widehat{G}$,

$$\begin{aligned}
 \langle e_l, e_k \rangle &= \frac{1}{|G|} \sum_{a \in G} e^{2\pi i \frac{l-k}{q} a} \\
 &= \begin{cases} 1 & l = k \\ 0 & l \neq k \end{cases}
 \end{aligned}$$

■

Thus, $|\widehat{G}| \leq |G|$. By carefully constructing maps from \widehat{G} to G , it can be shown that $|\widehat{G}| \geq |G|$. Hence the theorem:

Theorem 1.7. $|\widehat{G}| = |G|$

Using the results proved above, we can state the orthogonality principles:

1. Let $e \in \widehat{G}$.

$$\sum_{g \in G} e(g) = \begin{cases} |G| & \text{if } e \text{ is the identity} \\ 0 & \text{otherwise} \end{cases}$$

2. Let $x \in G$.

$$\sum_{e \in \widehat{G}} e(x) = \begin{cases} |G| & \text{if } x \text{ is the identity} \\ 0 & \text{otherwise} \end{cases}$$

▲▼▲

Chapter 2

Analytic Theory



Chapter 3

Advanced Topics



References

- [Apostol, 1976] Apostol, T. M. (1976). *Introduction to Analytic Number Theory*. Undergraduate Texts in Mathematics. Springer.
- [Murty, 2008] Murty, M. R. (2008). *Problems in Analytic Number Theory*. Graduate Texts in Mathematics. Springer.
- [Nathanson, 2000] Nathanson, M. B. (2000). *Elementary Methods in Number Theory*. Graduate Texts in Mathematics. Springer.